Coq/src/SimRelCont.v
@@ -4,7 +4,7 @@ From promising Require Import Basic.
 From imm Require Import Events Execution TraversalConfig Traversal
      Prog ProgToExecution ProgToExecutionProperties imm_s imm_s_hb 
      CombRelations SimTraversal SimulationRel AuxRel.
-Require Import AuxRel AuxDef EventStructure Consistency Construction EventToAction LblStep.
+Require Import AuxRel AuxDef EventStructure Consistency BasicStep EventToAction LblStep.
 
 Set Implicit Arguments.
 Local Open Scope program_scope.
@@ -197,7 +197,7 @@ Section EventToActionLemmas.
 
   (* Lemma basic_step_e2a_eq_dom e e' S' *)
   (*       (WF : ES.Wf S) *)
-  (*       (BSTEP : ESstep.t_basic e e' S S') : *)
+  (*       (BSTEP : ESBasicStep.t e e' S S') : *)
   (*   eq_dom (SE S) (e2a S') (e2a S). *)
   (* Proof. *)
   (*   cdes BSTEP; cdes BSTEP_. *)
@@ -276,12 +276,12 @@ Section SimRelContLemmas.
 
   Lemma basic_step_simrel_cont k k' e e' S'
         (st st' : thread_st (ES.cont_thread S k))
-        (BSTEP_ : ESstep.t_basic_ (cont_lang S k) k k' st st' e e' S S')
+        (BSTEP_ : ESBasicStep.t_ (cont_lang S k) k k' st st' e e' S S')
         (STCOV : C ∩₁ Gtid_ (ES.cont_thread S k) ⊆₁ acts_set st.(ProgToExecution.G)) : 
     simrel_cont prog S' G TC.
   Proof. 
     cdes BSTEP_.
-    assert (ESstep.t_basic e e' S S') as BSTEP.
+    assert (ESBasicStep.t e e' S S') as BSTEP.
     { econstructor; eauto. }
 
     assert (Stid S' (opt_ext e e') = ES.cont_thread S k) as TIDee.
@@ -457,11 +457,11 @@ Section SimRelContLemmas.
 
   (* Lemma basic_step_e2a_e k k' e e' S'  *)
   (*       (st st' : thread_st (ES.cont_thread S k)) *)
-  (*       (BSTEP_ : ESstep.t_basic_ (cont_lang S k) k k' st st' e e' S S') : *)
+  (*       (BSTEP_ : ESBasicStep.t_ (cont_lang S k) k k' st st' e e' S S') : *)
   (*   e2a S' e = ThreadEvent (ES.cont_thread S k) (st.(eindex)). *)
   (* Proof.  *)
   (*   cdes BSTEP_. *)
-  (*   assert (ESstep.t_basic e e' S S') as BSTEP. *)
+  (*   assert (ESBasicStep.t e e' S S') as BSTEP. *)
   (*   { econstructor; eauto. } *)
   (*   assert (SE S' e) as SEe.  *)
   (*   { eapply ESstep.basic_step_acts_set; eauto. basic_solver. } *)
@@ -483,11 +483,11 @@ Section SimRelContLemmas.
 
   (* Lemma basic_step_e2a_e' k k' e e' S'  *)
   (*       (st st' : thread_st (ES.cont_thread S k)) *)
-  (*       (BSTEP_ : ESstep.t_basic_ (cont_lang S k) k k' st st' e (Some e') S S') : *)
+  (*       (BSTEP_ : ESBasicStep.t_ (cont_lang S k) k k' st st' e (Some e') S S') : *)
   (*   e2a S' e' = ThreadEvent (ES.cont_thread S k) (1 + st.(eindex)). *)
   (* Proof.  *)
   (*   cdes BSTEP_. *)
-  (*   assert (ESstep.t_basic e (Some e') S S') as BSTEP. *)
+  (*   assert (ESBasicStep.t e (Some e') S S') as BSTEP. *)
   (*   { econstructor; eauto. } *)
   (*   assert (SE S' e') as SEe'.  *)
   (*   { eapply ESstep.basic_step_acts_set; eauto. basic_solver. } *)
