Coq/src/Step.v
@@ -1,0 +1,58 @@
+Require Import Omega.
+From hahn Require Import Hahn.
+From promising Require Import Basic.
+From imm Require Import Events AuxRel. 
+Require Import AuxRel AuxDef EventStructure Consistency.
+
+Set Implicit Arguments.
+
+Export ListNotations.
+
+Module ESstep.
+
+Notation "'E' S" := S.(ES.acts_set) (at level 10).
+Notation "'Einit' S"  := S.(ES.acts_init_set) (at level 10).
+Notation "'Eninit' S" := S.(ES.acts_ninit_set) (at level 10).
+
+Notation "'tid' S" := S.(ES.tid) (at level 10).
+Notation "'lab' S" := S.(ES.lab) (at level 10).
+Notation "'loc' S" := (Events.loc S.(ES.lab)) (at level 10).
+Notation "'mod' S" := (Events.mod S.(ES.lab)) (at level 10).
+
+Notation "'sb' S" := S.(ES.sb) (at level 10).
+Notation "'rmw' S" := S.(ES.rmw) (at level 10).
+Notation "'ew' S" := S.(ES.ew) (at level 10).
+Notation "'jf' S" := S.(ES.jf) (at level 10).
+Notation "'rf' S" := S.(ES.rf) (at level 10).
+Notation "'co' S" := S.(ES.co) (at level 10).
+Notation "'cf' S" := S.(ES.cf) (at level 10).
+
+Notation "'jfe' S" := S.(ES.jfe) (at level 10).
+Notation "'rfe' S" := S.(ES.rfe) (at level 10).
+Notation "'coe' S" := S.(ES.coe) (at level 10).
+Notation "'jfi' S" := S.(ES.jfi) (at level 10).
+Notation "'rfi' S" := S.(ES.rfi) (at level 10).
+Notation "'coi' S" := S.(ES.coi) (at level 10).
+
+Notation "'R' S" := (fun a => is_true (is_r S.(ES.lab) a)) (at level 10).
+Notation "'W' S" := (fun a => is_true (is_w S.(ES.lab) a)) (at level 10).
+Notation "'F' S" := (fun a => is_true (is_f S.(ES.lab) a)) (at level 10).
+
+Notation "'RW' S" := (R S ∪₁ W S) (at level 10).
+Notation "'FR' S" := (F S ∪₁ R S) (at level 10).
+Notation "'FW' S" := (F S ∪₁ W S) (at level 10).
+
+Notation "'Pln' S" := (fun a => is_true (is_only_pln S.(ES.lab) a)) (at level 10).
+Notation "'Rlx' S" := (fun a => is_true (is_rlx S.(ES.lab) a)) (at level 10).
+Notation "'Rel' S" := (fun a => is_true (is_rel S.(ES.lab) a)) (at level 10).
+Notation "'Acq' S" := (fun a => is_true (is_acq S.(ES.lab) a)) (at level 10).
+Notation "'Acqrel' S" := (fun a => is_true (is_acqrel S.(ES.lab) a)) (at level 10).
+Notation "'Sc' S" := (fun a => is_true (is_sc S.(ES.lab) a)) (at level 10).
+
+Notation "'same_loc' S" := (same_loc S.(ES.lab)) (at level 10).
+Notation "'same_val' S" := (same_val S.(ES.lab)) (at level 10).
+
+Notation "'K' S" := (S.(ES.cont_set)) (at level 10).
+
+Notation "'Tid' S" := (fun t e => S.(ES.tid) e = t) (at level 9).
+
